Instantiate compiler model with new importable&exportable

io/Compiler.Model.fst
@@ -15,21 +15,21 @@ open Compile.IIO.To.ILang
 (** *** IIO interface **)
 noeq
 type iio_interface = {
-  ct : erased tflag -> Type;
   pt : Type;
+  ct : erased tflag -> Type;
 
   ct_rc : tree pck_rc;
   pt_rc : tree pck_rc;
 
   ipi : monitorable_prop;
 
-  pt_exportable : fl:erased tflag -> exportable pt ipi pt_rc fl;
+  pt_exportable : exportable pt ipi pt_rc AllActions;
   ct_importable : fl:erased tflag -> importable (ct fl) ipi ct_rc fl;
 }
 
-let make_all_rc_eff (i:iio_interface) : typ_posts AllActions i.ct_rc =
-  let r : tree (pck_eff_rc AllActions) = map_tree i.ct_rc make_rc_eff in
-  assume (equal_trees i.ct_rc (map_tree r dfst));
+let make_all_rc_eff (rcs:tree pck_rc) : typ_posts AllActions rcs =
+  let r : tree (pck_eff_rc AllActions) = map_tree rcs make_rc_eff in
+  assume (equal_trees rcs (map_tree r dfst));
   r
 
 type ctx_iio (i:iio_interface) = #fl:erased tflag -> typ_posts fl i.ct_rc -> i.ct fl 
@@ -44,7 +44,7 @@ let iio_language : language = {
   whole = (i:iio_interface & i.pt);
 
   link = (fun #i p c -> 
-    let eff_rc = make_all_rc_eff i in
+    let eff_rc = make_all_rc_eff i.ct_rc in
     (| i, p (c #AllActions eff_rc) |));
   event_typ = IO.Sig.event;
 
@@ -79,104 +79,31 @@ let ilang_language : language = {
   beh = admit ();
 }
 
-(** *** RILang interface **)
-noeq
-type rilang_interface = {
-  pt : Type;
-  ct : Type;
-
-  ipi : monitorable_prop;
-  
-  pt_rilang : rilang pt ipi;
-  ct_rilang : rilang ct ipi;
-}
-
-type rilang_ctx (i:rilang_interface) = i.ct
-type rilang_prog (i:rilang_interface) = rilang_ctx i -> i.pt
-
-let rilang_language : language = {
-  interface = rilang_interface;
-
-  ctx = rilang_ctx;
-  pprog = rilang_prog;
-  whole = (i:rilang_interface & i.pt);
-
-  link = (fun #i p c -> (| i, p c |));
-  event_typ = IO.Sig.event;
-
-  beh = admit ();
-}
-
-(** *** TLang interface **)
-noeq
-type tlang_interface = {
-  pt : Type u#a;
-  ct : (Type u#b ->Type u#(max 1 b))->Type;
-
-  ipi : monitorable_prop;
-  
-  pt_rilang : rilang pt ipi;
-  ct_rilang : rilang (ct (dm_mon ipi).m) ipi;
-}
-
-type tlang_ctx (i:tlang_interface) = mon:monad -> acts mon -> i.ct mon.m
-type tlang_prog (i:tlang_interface) = i.ct ((dm_mon i.ipi).m) -> i.pt
-
-let tlang_language : language = {
-  interface = tlang_interface;
-
-  ctx = tlang_ctx;
-  pprog = tlang_prog;
-  whole = (i:tlang_interface & i.pt);
-
-  link = (fun #i p c -> (| i, p (c (dm_mon i.ipi) (dm_acts i.ipi)) |));
-  event_typ = IO.Sig.event;
-
-  beh = admit ();
-}
-
 (** ** Compile interfaces **)
-let comp_int_iio_ilang (i:iio_lang_interface) : ilang_interface = {
-    pt = resexn i.pt_exportable.etype;
-    ct = i.ct_importable.itype;
-    ipi = i.ipi;
+let comp_int_iio_ilang (i:iio_interface) : ilang_interface = {
+  pt = resexn i.pt_exportable.etype;
+  ct = (fun fl -> (i.ct_importable fl).itype);
+  ipi = i.ipi;
 
-    pt_ilang = ilang_resexn i.ipi i.pt_exportable.etype #i.pt_exportable.c_etype;
-    ct_ilang = i.ct_importable.c_itype;
-
-    pt_reifiable = reify_resexn i.ipi i.pt_exportable.etype #i.pt_reifiable;
-    ct_reflectable = i.ct_reflectable; 
+  pt_ilang = ilang_resexn i.ipi i.pt_exportable.etype #i.pt_exportable.c_etype;
+  ct_ilang = (fun fl -> (i.ct_importable fl).c_itype);
 }
 
-let comp_int_ilang_rilang (i:ilang_interface) : rilang_interface = {
-    pt = i.pt_reifiable.reify_out;
-    ct = i.ct_reflectable.reflect_in;
-    ipi = i.ipi;
-
-    pt_rilang = i.pt_reifiable.rilang_reify_out;
-    ct_rilang = i.ct_reflectable.rilang_reflect_in;
-}
-
-let comp_int_rilang_tlang (i:rilang_interface) : tlang_interface = {
-    pt = i.pt;
-    ct = (fun m -> i.ct); // is this ok?
-    ipi = i.ipi;
-
-    pt_rilang = i.pt_rilang;
-    ct_rilang = i.ct_rilang; // I suppose yes because of this constraint
-}
 
 (** ** Phases of compilation **)
-let compiler_pprog_iio_ilang (#i:iio_lang_interface) (p_s:iio_lang_language.pprog i) : ilang_language.pprog (comp_int_iio_ilang i) = fun c_t -> 
-    match i.ct_importable.import c_t with
-    | Inl c_s -> begin 
-      let (| _, ws |) = iio_lang_language.link #i p_s c_s in
-      Inl (i.pt_exportable.export ws)
+let compiler_pprog_iio_ilang (#i:iio_interface) (p_s:prog_iio i) : ilang_language.pprog (comp_int_iio_ilang i) = 
+  fun c_t -> 
+    let eff_rc = make_all_rc_eff i.ct_rc in
+    match (i.ct_importable AllActions).import c_t eff_rc with
+    | Inl (c_s:i.ct AllActions) -> begin
+       let p : i.pt = p_s c_s in
+       let eff_rc = make_all_rc_eff i.pt_rc in
+       Inl (i.pt_exportable.export eff_rc p)
     end
     | Inr err -> Inr err
 
 let phase1 : compiler = {
-  source = iio_lang_language;
+  source = iio_language;
   target = ilang_language;
 
   comp_int = comp_int_iio_ilang;
@@ -186,52 +113,24 @@ let phase1 : compiler = {
   rel_traces = (==);
 }
 
-let compiler_pprog_ilang_rilang (#i:ilang_interface) (p_s:ilang_language.pprog i) : rilang_language.pprog (comp_int_ilang_rilang i) = fun c_t -> 
-  let c_s = i.ct_reflectable._reflect c_t in
-  let (| _, ws |) = ilang_language.link #i p_s c_s in
-  i.pt_reifiable._reify ws
-
-let phase2 : compiler = {
-  source = ilang_language;
-  target = rilang_language;
-
-  comp_int = comp_int_ilang_rilang;
-
-  compile_pprog = compiler_pprog_ilang_rilang;
-
-  rel_traces = (==);
-}
-
-let compiler_pprog_rilang_tlang (#i:rilang_interface) (p_s:rilang_language.pprog i) : tlang_language.pprog (comp_int_rilang_tlang i) = p_s
-
-let phase3 : compiler = {
-  source = rilang_language;
-  target = tlang_language;
-
-  comp_int = comp_int_rilang_tlang;
-
-  compile_pprog = compiler_pprog_rilang_tlang;
-
-  rel_traces = (==);
-}
-
-let compiler = (phase1 `chain_compilers` phase2) `chain_compilers` phase3
+open FStar.List
 
 (** Tests **)
-let test_interface : iio_lang_interface = {
-  pt = unit -> IIO unit (fun h -> True) (fun h r lt -> True);
-  ct = (x:file_descr) -> IIO unit (fun h -> is_open x h) (fun h r lt -> is_open x (apply_changes h lt));
-
+let test_interface : iio_interface = {
   ipi = (fun _ _ _ -> true);
 
-  pt_exportable = admit ();
-  ct_importable = admit ();
-  pt_reifiable = admit ();
-  ct_reflectable = admit ();
+  pt = unit -> IIOpi (resexn unit) AllActions (fun _ _ _ -> true);
+  pt_rc = EmptyNode Leaf Leaf;
+
+  ct = (fun fl -> unit -> IIO (resexn file_descr) fl (fun _ -> True) (fun h rfd lt -> Inl? rfd ==> is_open (Inl?.v rfd) (rev lt @ h)));
+  ct_rc = Node (| unit, resexn file_descr, (fun () h (rfd:resexn file_descr) lt -> Inl? rfd && (is_open (Inl?.v rfd) (rev lt @ h))) |) Leaf Leaf;
+
+
+  pt_exportable = exportable_arrow_with_no_pre_and_no_post unit #importable_unit unit #exportable_unit;
+  ct_importable = admit () //safe_importable_is_importable (safe_importable_arrow_pre_post file_descr unit );
 }
 
-val test_prog : iio_lang_prog test_interface
-let test_prog ctx () =
-  let fd = static_cmd Openfile "../Makefile" in
-  if Inl? fd then ctx (Inl?.v fd)
-  else ()
+val test_prog : prog_iio test_interface
+let test_prog ctx () : IIOpi (resexn unit) AllActions (fun _ _ _ -> true) by (unfold_def (`pi_as_hist); unfold_def (`hist_return); explode (); bump_nth 3; dump "H") =
+  let _ = ctx () in
+  Inl ()
